Prove unsafe_get and get.

rocq-osiris/theories/program_logic/reasoning_rules/array_rules.v
@@ -1,102 +1,139 @@
 From iris Require Import gen_heap proofmode.proofmode.
 From osiris Require Import lang.
 From osiris.program_logic Require Import ewp.
-From osiris.program_logic.reasoning_rules Require Import basic_rules stop_rules expr_rules.
+From osiris.program_logic.reasoning_rules Require Import impure_rules stop_rules.
 
 Section array_resources.
 
   Context `{!osirisGS Σ}.
 
-  Definition isArray (a : val) (n : nat) : iProp Σ :=
+  Definition isArray (a : val) (n : Z) : iProp Σ :=
     ∃ (ls : list loc),
       ⌜a = VArray ls⌝ ∗
-      ⌜length ls = n⌝ ∗
-      ⌜Z.of_nat n < max_array⌝.
+      ⌜length ls = Z.to_nat n⌝ ∗
+      ⌜0 ≤ n < max_array⌝.
 
   Global Instance is_array_persistent a n : Persistent (isArray a n).
   Proof. apply _. Qed.
 
-  Definition isSlice `{Encode A} dq (a : val) (i : nat) (xs : list A) : iProp Σ :=
+  Definition isSlice `{Encode A} dq (a : val) (i : Z) (xs : list A) : iProp Σ :=
     ∃ (ls : list loc),
-      ⌜a = VArray ls⌝ ∗ ⌜(i + length xs ≤ length ls)%nat⌝ ∗
-      [∗ list] l;x ∈ take (length xs) (drop i ls); xs, pointsto l dq (V #x).
+      ⌜a = VArray ls⌝ ∗ ⌜0 ≤ i ∧ i + length xs ≤ length ls⌝ ∗
+      [∗ list] l;x ∈ take (length xs) (drop (Z.to_nat i) ls); xs, pointsto l dq (V #x).
 
-  Lemma leq_length {A} i (l : list A) :
-    (i ≤ length l)%nat →
+  Lemma leq_length {A} (i : Z) (l : list A) :
+    0 ≤ i ≤ length l →
     ∃ li lrest, l = li ++ lrest ∧ i = length li.
   Proof.
-    intros Hle.
-    exists (take i l), (drop i l).
-    split. by rewrite take_drop. rewrite length_take. lia.
+    intros [Hpos Hle].
+    exists (take (Z.to_nat i) l), (drop (Z.to_nat i) l).
+    split. by rewrite take_drop. rewrite length_take.
+    assert (Z.to_nat i `min` length l = Z.to_nat i)%nat as -> by lia.
+    rewrite Z2Nat.id; [ reflexivity | assumption ].
   Qed.
 
-  Lemma eq_length {A} i j (l : list A) :
-    (i + j = length l)%nat →
+  Lemma eq_length {A} (i j : Z) (l : list A) :
+    0 ≤ i ∧ 0 ≤ j →
+    i + j = length l →
     ∃ li lj, l = li ++ lj ∧ i = length li ∧ j = length lj.
   Proof.
-    intros Heq.
-    exists (take i l), (drop i l).
+    intros Hpos Heq.
+    exists (take (Z.to_nat i) l), (drop (Z.to_nat i) l).
     split. by rewrite take_drop. rewrite length_take length_drop. lia.
   Qed.
 
-  Local Lemma decompose_list {A} i j k (ls : list A) :
-    (i + j + k ≤ length ls)%nat →
+  Local Lemma decompose_list {A} (i j k : Z) (ls : list A) :
+    (0 ≤ i ∧ 0 ≤ j ∧ 0 ≤ k) →
+    (i + j + k ≤ length ls) →
     ∃ li lys lzs lextra,
       ls = li ++ lys ++ lzs ++ lextra ∧
       i = length li ∧ j = length lys ∧ k = length lzs.
   Proof.
-    intros constraint.
-    apply leq_length in constraint as (l' & lextra & -> & Hlen).
-    apply eq_length in Hlen as (l1 & l2 & -> & Hlen1 & Hlen2).
-    apply eq_length in Hlen1 as (l1' & l2' & -> & Hlen1' & Hlen2').
+    intros Hpos constraint.
+    assert (0 ≤ i + j + k ∧ i + j + k ≤ length ls) as Hpos' by lia.
+    apply leq_length in Hpos' as (l' & lextra & -> & Hlen).
+    apply eq_length in Hlen as (l1 & l2 & -> & Hlen1 & Hlen2); last lia.
+    apply eq_length in Hlen1 as (l1' & l2' & -> & Hlen1' & Hlen2'); last lia.
     exists l1', l2', l2, lextra.
     rewrite !app_assoc. auto.
-   Qed.
+  Qed.
 
-   Lemma split_Slice `{Encode A} dq a (i j : nat) (xs ys zs : list A) :
-     j = (i + length ys)%nat →
+  Local Lemma cut_out_slice {A} (i j : Z) (ls : list A) :
+    (0 ≤ i ∧ 0 ≤ j) →
+    (i + j ≤ length ls) →
+    ∃ li slice lextra,
+      ls = li ++ slice ++ lextra ∧
+      i = length li ∧ j = length slice.
+  Proof.
+    intros Hpos constraint.
+    assert (0 ≤ i + j ∧ i + j ≤ length ls) as Hpos' by lia.
+    apply leq_length in Hpos' as (l' & lextra & -> & Hlen).
+    apply eq_length in Hlen as (l1 & l2 & -> & Hlen1 & Hlen2); last lia.
+    exists l1, l2, lextra. rewrite app_assoc. auto.
+  Qed.
+
+   Lemma split_Slice `{Encode A} dq a (i j : Z) (xs ys zs : list A) :
+     j = i + length ys →
      xs = ys ++ zs →
      isSlice dq a i xs ⊣⊢ (isSlice dq a i ys ∗ isSlice dq a j zs).
    Proof.
      intros -> ->.
      iStartProof; iSplit; iIntros "Hslice".
-     - iDestruct "Hslice" as "(%ls & -> & %Hlen & Hslice)".
-       rewrite length_app Nat.add_assoc in Hlen.
+     - iDestruct "Hslice" as "(%ls & -> & [%Hpos %Hlen] & Hslice)".
+       rewrite length_app in Hlen.
+       replace (i + (length ys + length zs)%nat)
+         with (i + length ys + length zs) in Hlen by lia.
        (* Decompose [ls] into [li ++ lys ++ lzs ++ lextra]. *)
-       destruct (decompose_list _ _ _ ls Hlen) as (li & lys & lzs & lextra & -> & Hlen1 & Hlen2 & Hlen3).
-       rewrite Hlen1 drop_app_length.
-       rewrite {1}app_assoc.
-       rewrite length_app. rewrite {1}Hlen2 {1}Hlen3. rewrite <- length_app.
+       assert (0 ≤ i ∧ 0 ≤ length ys ∧ 0 ≤ length zs) as Hpos' by lia.
+       destruct (decompose_list _ _ _ ls Hpos' Hlen)
+         as (li & lys & lzs & lextra & -> & Hlen1 & Hlen2 & Hlen3).
+       replace (Z.to_nat i) with (length li) by lia.
+       rewrite drop_app_length {1} app_assoc.
+       rewrite length_app.
+       replace (length ys) with (length lys) by lia.
+       replace (length zs) with (length lzs) by lia.
+       rewrite <- length_app.
        rewrite take_app_length.
-       iPoseProof (big_sepL2_app_inv with "Hslice") as "[Hslice1 Hslice2]". auto.
+       iPoseProof (big_sepL2_app_inv with "Hslice") as "[Hslice1 Hslice2]". lia.
        iSplitL "Hslice1".
        + iExists _. iSplit; first done. iSplit.
          { iPureIntro. rewrite !length_app. lia. }
-         rewrite drop_app_length. rewrite Hlen2.
-         rewrite take_app_length. iApply "Hslice1".
+         replace (Z.to_nat i) with (length li) by lia.
+         rewrite drop_app_length.
+         replace (length ys) with (length lys) by lia.
+         rewrite take_app_length.
+         iApply "Hslice1".
        + iExists _. iSplit; first done. iSplit.
          { iPureIntro. rewrite !length_app. lia. }
-         rewrite Hlen2.
+         replace (length zs) with (length lzs) by lia.
+         replace (Z.to_nat (i + length lys)) with (length li + length lys)%nat by lia.
          rewrite <- (length_app li lys).
-         rewrite app_assoc drop_app_length.
-         rewrite Hlen3 take_app_length. iApply "Hslice2".
+         rewrite app_assoc drop_app_length take_app_length.
+         iApply "Hslice2".
      - iDestruct "Hslice" as "(Hslice1 & Hslice2)".
-       iDestruct "Hslice1" as "(%ls & %Harr & %Hlen & Hslice1)".
-       iDestruct "Hslice2" as "(%ls' & %Harr' & %Hlen' & Hslice2)".
-       rewrite Harr' in Harr. inversion Harr; subst.
+       iDestruct "Hslice1" as "(%ls & %Harr & [%Hpos %Hlen] & Hslice1)".
+       iDestruct "Hslice2" as "(%ls' & %Harr' & [%Hpos' %Hlen'] & Hslice2)".
+       rewrite Harr' in Harr; inversion Harr; subst.
        iExists ls. iSplit; first done. iSplit.
        { iPureIntro. rewrite length_app. lia. }
        (* Decompose [ls] into [li ++ lys ++ lzs ++ lextra]. *)
-       destruct (decompose_list _ _ _ ls Hlen') as (li & lys & lzs & lextra & -> & Hlen1 & Hlen2 & Hlen3).
-       rewrite Hlen1 drop_app_length.
-       rewrite length_app Hlen2 Hlen3. rewrite <- !length_app.
+       assert (0 ≤ i ∧ 0 ≤ length ys ∧ 0 ≤ length zs) as Hpos'' by lia.
+       destruct (decompose_list _ _ _ ls Hpos'' Hlen')
+         as (li & lys & lzs & lextra & -> & Hlen1 & Hlen2 & Hlen3).
+       replace (Z.to_nat i) with (length li) by lia.
+       replace (Z.to_nat (i + length ys)) with (length li + length ys)%nat by lia.
+       rewrite length_app.
+       replace (length ys) with (length lys) by lia.
+       replace (length zs) with (length lzs) by lia.
+       rewrite <- !length_app. rewrite !drop_app_length.
        rewrite {3}app_assoc !take_app_length.
        iApply (big_sepL2_app with "Hslice1 [Hslice2]").
        rewrite app_assoc drop_app_length take_app_length.
        iApply "Hslice2".
    Qed.
 
-   Definition isArrayCell `{Encode A} dq (a : val) (i : nat) (x : A) : iProp Σ := isSlice dq a i [x].
+   Definition isArrayCell `{Encode A} dq (a : val) (i : nat) (x : A) : iProp Σ :=
+     isSlice dq a i [x].
 
  End array_resources.
 
@@ -106,63 +143,81 @@ Section array_resources.
 
    Context {ι : thread} {η : env} {E : coPset} {Ψ : iEff Σ}.
 
-   Lemma ewp_EArrayLength n e :
-     EWP[ι] eval η e @ E <|Ψ|> {{ ensures a, isArray a n }} -∗
-     EWP[ι] eval η (EArrayLength e) @ E <|Ψ|> {{ ensures #n', ⌜n' = n⌝ }}.
+   Lemma imp_EArrayLength {ζ} (n : Z) e :
+     imp^{ι} eval η e @ E <|Ψ|> ⟨⟨ ζ ⟩⟩ {{ λ a, isArray a n }} -∗
+     imp^{ι} eval η (EArrayLength e) @ E <|Ψ|> ⟨⟨ ζ ⟩⟩ {{ λ n', ⌜n' = n⌝ }}.
    Proof.
-     iIntros "He".
-     simpl_eval.
-     iApply ewp_bind.
-     iApply ewp_bind.
-     iApply (ewp_mono with "He").
-     iIntros ([|]); [ | iIntros ([]) ].
-     iIntros "#Harray". simpl.
-     iDestruct "Harray" as "(%ls & -> & %Hlen & %Hbound)".
-     iApply ewp_ret. iApply ewp_ret.
-     iExists n. rewrite Hlen.
-     auto.
+     iIntros "He". simpl_eval.
+     iApply (imp_bind _ _ (λ ls, ret (VInt (repr (length ls)))) with "[He]").
+     { rewrite /as_array.
+       iApply (imp_bind _ _ (λ v, val_as_array v) with "He").
+       iIntros (a) "#Harray".
+       iDestruct "Harray" as "(%ls & -> & Harray)". simpl.
+       iApply (imp_ret ls ls).
+       instantiate (1 := Build_Observe (list loc) _ (list loc) id). reflexivity.
+       iExact "Harray". }
+     iIntros (ls) "(%Hlen & %Hbound)".
+     change (♯ls) with ls.
+     iApply (imp_ret (VInt (repr (length ls))) (Z.of_nat (length ls))%Z). encode.
+     iPureIntro. lia.
    Qed.
 
-   Lemma ewp_EArrayMake `{Encode A} {e1 e2} n (φ : A → iProp Σ) :
-     ⌜Z.of_nat n < max_array⌝ -∗
-     EWP[ι] eval η e1 @ E <|Ψ|> {{ ensures #i, ⌜i=n⌝ }} -∗
-     EWP[ι] eval η e2 @ E <|Ψ|> {{ ensures #x, φ x }} -∗
-     EWP[ι] eval η (EArrayMake e1 e2) @ E <|Ψ|>
-       {{ ensures a, ∃ x, φ x ∗ isArray a n ∗ isSlice (DfracOwn 1) a 0 (repeat x n) }}.
+   Lemma array_size_representable i :
+     0 ≤ i < max_array →
+     representable i.
    Proof.
-     iIntros (Hbound) "He1 He2".
-     simpl_eval.
-     iApply (ewp_Par with "[He1] He2").
-     - iApply ewp_bind. iApply (ewp_mono with "He1").
-       iIntros ([|]); [ | iIntros ([]) ].
-       iIntros "(%v & -> & ->) /=".
-       rewrite (signed_repr n).
-       assert (n >=? 0 = true) as -> by apply Z.geb_le, Nat2Z.is_nonneg.
-       iApply ewp_ret.
-       instantiate (1 := (λ o, match o with O2Ret i => ⌜i = n⌝ | O2Throw _ => False end)%I).
-       simpl. iPureIntro. apply Nat2Z.id.
-       pose proof (h := (Z.lt_trans n max_array max_signed Hbound max_array_length)).
-       constructor; last lia.
-       transitivity 0. rewrite min_signed_eq.
+     intros (Hpos & Hlt).
+     constructor.
+     - rewrite min_signed_eq.
+       transitivity 0; last assumption.
        apply Z.opp_nonpos_nonneg. apply Z.lt_le_incl, Z.gt_lt.
        apply Coqlib.two_power_nat_pos.
-       apply Nat2Z.is_nonneg.
-     - iIntros (? []).
-     - iIntros (? []).
-     - iIntros (i a ->) "Hφ".
-       iNext. iApply ewp_bind. iApply ewp_ret. simpl.
-       assert (n <? max_array = true) as -> by apply Z.ltb_lt, Hbound.
-       iApply ewp_allocn.
+     - pose proof (h := (Z.lt_trans i max_array max_signed Hlt max_array_length)).
+       apply Z.lt_le_incl, h.
+   Qed.
+
+   Lemma imp_EArrayMake `{Encode A} {ζ} {e1 e2} (n : Z) (Φ : A → iProp Σ) :
+     ⌜0 ≤ n < max_array⌝ -∗
+     imp^{ι} eval η e1 @ E <|Ψ|> ⟨⟨ ζ ⟩⟩ {{ λ i, ⌜i = n⌝ }} -∗
+     imp^{ι} eval η e2 @ E <|Ψ|> ⟨⟨ ζ ⟩⟩ {{ Φ }} -∗
+     imp^{ι} eval η (EArrayMake e1 e2) @ E <|Ψ|> ⟨⟨ ζ ⟩⟩
+       {{ λ a, ∃ x, Φ x ∗ isArray a n ∗ isSlice (DfracOwn 1) a 0 (repeat x (Z.to_nat n)) }}.
+   Proof.
+     iIntros (Hbound) "He1 He2". simpl_eval.
+     iApply (@imp_Par _ _ val val exn _ _
+               _ _ _ _ _ _ _ _ _ _ _ _ _ _
+               _ _ _ _ (as_int (eval η e1)) _ (pfbind inject2
+               (λ '(n0, v),
+                  if ((0 <=? signed n0) && (signed n0 <? max_array))%bool
+                  then
+                   Stop CAllocn (Z.to_nat (signed n0), v)
+                     (pfbind inject2 (λ ls : list loc, ret (VArray ls)))
+                  else throw (invalid_argument "Array.make"))) with "[He1] He2").
+     { rewrite /as_int.
+       iApply (imp_bind _ _ (λ v, val_as_int v) with "He1").
+       iIntros (?) "-> /=".
+       iApply (imp_ret (repr n) n). instantiate (1 := Build_Observe Z _ int repr). reflexivity.
+       instantiate (1 := (λ i, ⌜i = n⌝)%I). done. }
+     iSplit; last iSplit.
+     - iIntros (e) "Hζ !>".
+       iApply (imp_throw with "Hζ").
+     - iIntros (e) "Hζ !>".
+       iApply (imp_throw with "Hζ").
+     - iIntros (? a) "-> Hφ !>".
+       rewrite /continue /=.
+       rewrite bind_ret.
+       rewrite signed_repr; last apply array_size_representable, Hbound.
+       assert (0 <=? n = true) as -> by lia.
+       assert (n <? max_array = true) as -> by lia.
+       iApply imp_allocn.
        iIntros "!>" (ls) "(%Hlen & Hpts)".
-       iApply ewp_ret. simpl.
-       iDestruct "Hφ" as "(%x & -> & Hφ)".
+       rewrite /continue /=.
+       iApply imp_ret. encode.
        iFrame.
-       iSplitR.
-       iExists ls; auto.
+       iSplitR. { iExists ls; auto. }
        iExists ls. iSplit; first done.
-       iSplit; first iPureIntro.
-       rewrite repeat_length. lia.
-       rewrite drop_0. rewrite repeat_length. rewrite <- Hlen, firstn_all.
+       iSplit; first (iPureIntro; rewrite repeat_length; lia).
+       rewrite drop_0 repeat_length. rewrite <- Hlen, firstn_all.
        iApply big_sepL2_alt.
        iSplit; first (iPureIntro; by rewrite repeat_length).
        clear Hlen.
@@ -173,83 +228,237 @@ Section array_resources.
          iApply ("IH" with "Hpts").
    Qed.
 
-   Lemma ewp_EArrayUnsafeGet `{Encode A} a (n : nat) (i j : nat) dq (xs : list A) x e1 e2 :
-     ⌜(0 ≤ i < n)%nat⌝ -∗
-     ⌜xs !! i = Some x⌝ -∗
-     isArray a n -∗
-     isSlice dq a j xs -∗
-     EWP[ι] eval η e1 @ E <|Ψ|> {{ ensures a', ⌜a' = a⌝ }} -∗
-     EWP[ι] eval η e2 @ E <|Ψ|> {{ ensures #i', ⌜i' = i⌝ }} -∗
-     EWP[ι] eval η (EArrayUnsafeGet e1 e2) @ E <|Ψ|> {{ ensures #v, ⌜v=x⌝ ∗ isSlice dq a j xs }}.
+   Lemma imp_EArrayUnsafeGet2 `{Encode A} {Φ : A → iProp Σ} {ζ} (Φ1 : val → iProp Σ) (Φ2 : Z → iProp Σ) e1 e2 :
+     imp^{ι} eval η e1 @ E <|Ψ|> ⟨⟨ ζ ⟩⟩ {{ λ a, ∃ n, isArray a n ∗ Φ1 a }} -∗
+     imp^{ι} eval η e2 @ E <|Ψ|> ⟨⟨ ζ ⟩⟩ {{ λ i, Φ2 i }} -∗
+     (∀ a i, Φ1 a -∗ Φ2 i -∗
+             ∃ n, isArray a n ∗
+             ∃ dq j xs x,
+               ▷ (⌜j ≤ i⌝ ∗ isSlice dq a j xs ∗ ⌜xs !! (i - j) = Some x⌝) ∗
+               ▷ (isSlice dq a j xs -∗ Φ x)) -∗
+     imp^{ι} eval η (EArrayUnsafeGet e1 e2) @ E <|Ψ|> ⟨⟨ ζ ⟩⟩ {{ Φ }}.
    Proof.
-     iIntros (Hi Hlookup) "#Harr Hslice He1 He2".
-     iDestruct "Hslice" as "(%ls & -> & %Hlen & Hslice)".
-     iDestruct "Harr" as "(%ls' & -> & %Hlen' & %Hbound)".
-     simpl_eval.
-     iApply (ewp_Par with "[He1] [He2]").
-     - iApply ewp_bind. iApply (ewp_mono with "He1").
-       iIntros ([|]); [ | iIntros ([]) ].
-       iIntros (->).
-       iApply ewp_ret.
-       instantiate (1 := (λ o, match o with O2Ret ls => ⌜ls = ls'⌝ | O2Throw _ => False end)%I).
-       auto.
-     - iApply ewp_bind. iApply (ewp_mono with "He2").
-       iIntros ([|]); [ | iIntros ([]) ].
-       iIntros "(%v & -> & ->) /=".
-       rewrite (signed_repr i).
-       assert (i >=? 0 = true) as -> by apply Z.geb_le, Nat2Z.is_nonneg.
-       iApply ewp_ret.
-       instantiate (1 := (λ o, match o with O2Ret i' => ⌜i' = i⌝ | O2Throw _ => False end)%I).
-       simpl. iPureIntro. apply Nat2Z.id.
-       constructor.
-       transitivity 0. rewrite min_signed_eq.
-       apply Z.opp_nonpos_nonneg. apply Z.lt_le_incl, Z.gt_lt.
-       apply Coqlib.two_power_nat_pos.
-       lia.
-       transitivity n. lia.
-       pose proof (h := (Z.lt_trans n max_array max_signed Hbound max_array_length)).
-       lia.
-     - iIntros (? []).
-     - iIntros (? []).
-     - iIntros (? ? -> ->).
-       iNext.
-       iApply ewp_bind. iApply ewp_ret. simpl.
-       admit.
-   Admitted.
+     iIntros "He1 He2 P". simpl_eval.
+     iApply (imp_Par _ _ _ _ _ _ (pfbind inject2
+               (λ '((ls0, i0) : list loc * int),
+                  match ls0 !! signed i0 with
+                  | Some l => load l
+                  | None => crash "index out of bounds"
+                  end)) with "[He1] [He2]").
+     { rewrite /as_array.
+       iApply (imp_bind _ _ (λ v, val_as_array v) with "He1").
+       iIntros (a) "(%n & (%ls & -> & Harr) & HΦ1)".
+       iApply (imp_ret ls ls).
+       instantiate (1 := Build_Observe (list loc) _ (list loc) id). reflexivity.
+       instantiate (1 := (λ ls', Φ1 (VArray ls'))%I). done. }
+     { rewrite /as_int.
+       iApply (imp_bind _ _ (λ v, val_as_int v) with "He2").
+       iIntros (i) "HΦ2".
+       iApply (imp_ret (repr i) i).
+       instantiate (1 := Build_Observe (Z) _ (int) repr). reflexivity.
+       iExact "HΦ2". }
+     iSplit; last iSplit.
+     { iIntros (e) "Hζ !>".
+       iApply (imp_throw with "Hζ"). }
+     { iIntros (e) "Hζ !>".
+       iApply (imp_throw with "Hζ"). }
+     iIntros (ls i) "HΦ1 HΦ2".
+     iDestruct ("P" with "HΦ1 HΦ2")
+       as "(%n & #Harr & %dq & %j & %xs & %x & P)".
+     rewrite /continue /= bind_ret.
+     iNext.
+     iDestruct "P" as "((%Hle & Hslice & %Hlookup) & P)".
 
-   Lemma ewp_EArrayGet `{Encode A} a (n : nat) (i : nat) e1 e2 φ :
-     isArray a n -∗
-     isSlice dq a j xs -∗
-     EWP[ι] eval η e1 @ E <|Ψ|> {{ ensures a', ⌜a' = a⌝ }} -∗
-     EWP[ι] eval η e2 @ E <|Ψ|> {{ ensures #i', ⌜i' = i⌝ }} -∗
-     (∀ a, ∃ dq (j : nat) (xs : list A),
-             isSlice dq a j xs ∗ ▷ (isSlice dq a j xs -∗ ∃ x, ⌜xs !! (i - j)%nat = Some x⌝ ∗ φ x)) -∗
-     EWP[ι] eval η (EArrayGet e1 e2) @ E <|Ψ|> {{ ensures #x, φ x }}.
-   Proof.
-     iIntros "#Harr He1 He2 Hmono".
-     simpl_eval.
-     iApply (ewp_Par with "[He1] [He2]").
-     - iApply ewp_bind. iApply (ewp_mono with "He1").
-       iIntros ([|]); [ | iIntros ([]) ].
-       iIntros (->). iDestruct "Harr" as "(%ls & -> & %Hlen & %Hbound)".
-       iApply ewp_ret.
-       instantiate (1 := (ensures ls, ∃ n, ⌜length ls = n⌝ ∗ ⌜n ≤ max_array⌝)%I).
-       iExists n; auto.
-     - iApply ewp_bind. iApply (ewp_mono with "He2").
-       iIntros ([|]); [ | iIntros ([]) ].
-       iIntros "(%v & -> & ->) /=".
+     iDestruct "Harr" as "(% & %Heq & %Hlen' & %Hbound)".
+     iDestruct "Hslice" as "(% & %Heq' & %Hlen & Hslice)".
+     inversion Heq; subst ls0; clear Heq.
+     inversion Heq'; subst ls1; clear Heq'.
 
+     (* Decompose [ls] into [lj ++ slice ++ _]. *)
+     pose proof (cut_out_slice j (length xs) ls ltac:(lia) ltac:(lia))
+       as (lj & slice & lextra & Hls & Hj & Hslice).
+     (* Turn [take _ (drop _ ls)] into [slice]. *)
+     replace (Z.to_nat j) with (length lj) by lia.
+     rewrite {1}Hls drop_app_length.
+     replace (length xs) with (length slice) by lia.
+     rewrite take_app_length.
 
-     iApply ewp_bind.
-     iApply (ewp_mono with "He").
-     iIntros ([|]); [ | iIntros ([]) ].
-     iIntros "#Harray". simpl.
-     iDestruct "Harray" as "(%ls & -> & %Hlen & %Hbound)".
-     iApply ewp_ret. iApply ewp_ret.
-     iExists n. rewrite Hlen.
-     auto.
+     rewrite /lookup /list_lookup_Z in Hlookup.
+     assert (i - j <? 0 = false) as Heqf by lia.
+     rewrite Heqf in Hlookup.
+
+     assert (i - j < length xs).
+     { pose proof (lookup_lt_Some xs (Z.to_nat (i - j)) _ Hlookup). lia. }
+     rewrite (signed_repr i); last (apply array_size_representable; lia).
+
+     (* [Decompose [xs] intl [xk ++ x :: _]. *)
+     pose proof (list_elem_of_split_length xs (Z.to_nat (i - j)) x Hlookup)
+       as (xk & xrest & Hxs & Hxk).
+     rewrite {1}Hxs.
+
+     (* Inversions on [Hslice] gives us that
+        [slice] = [slicek ++ l :: _]. *)
+     iDestruct (big_sepL2_app_inv_r with "Hslice")
+       as "(%slicek & %slice' & -> & Hslice1 & Hslice2)".
+     iDestruct (big_sepL2_cons_inv_r with "Hslice2") as
+       "(%l & %slicerest & -> & Hl & Hslice2)".
+
+     (* We can now prove that [ls !! Z.to_nat i] = [Some l]. *)
+     rewrite /lookup /list_lookup_Z.
+     assert (i <? 0 = false) as -> by lia.
+     rewrite {2}Hls lookup_app_r; last lia.
+     replace (Z.to_nat i - length lj)%nat with (Z.to_nat (i - j)) by lia.
+     rewrite <- app_assoc. iPoseProof (big_sepL2_length with "Hslice1") as "%Hleneq".
+     rewrite list_lookup_middle; last lia.
+
+     iApply (imp_load with "Hl").
+     rewrite /continue; iIntros "!> Hl /=".
+     iApply imp_ret. encode. iApply "P".
+     iCombine ("Hl Hslice2") as "Hslice2".
+     iPoseProof (big_sepL2_cons (λ _ l' x', pointsto l' dq (V #x')) with "Hslice2") as "Hslice2".
+     iPoseProof (big_sepL2_app with "Hslice1 Hslice2") as "Hslice".
+     iExists ls. iSplit; first auto. iSplit.
+     { iPureIntro. lia. }
+     replace (Z.to_nat j) with (length lj) by lia.
+     rewrite {1}Hls drop_app_length.
+     replace (length xs) with (length (slicek ++ l :: slicerest)) by lia.
+     rewrite take_app_length.
+     rewrite Hxs.
+     iApply "Hslice".
    Qed.
 
+   Lemma imp_EArrayUnsafeGet `{Encode A} {ζ} a (k n : Z) (i j : Z) dq (xs : list A) x e1 e2 :
+     ⌜j ≤ i⌝ -∗
+     ⌜xs !! (i - j)%Z = Some x⌝ -∗
+     isArray a n -∗
+     ▷ isSlice dq a j xs -∗
+     imp^{ι} eval η e1 @ E <|Ψ|> ⟨⟨ ζ ⟩⟩ {{ λ a', ⌜a' = a⌝ }} -∗
+     imp^{ι} eval η e2 @ E <|Ψ|> ⟨⟨ ζ ⟩⟩ {{ λ i', ⌜i' = i⌝ }} -∗
+     imp^{ι} eval η (EArrayUnsafeGet e1 e2) @ E <|Ψ|> ⟨⟨ ζ ⟩⟩
+           {{ λ v, ⌜v = x⌝ ∗ isSlice dq a j xs }}.
+   Proof.
+     iIntros (Hi Hlookup) "#Harr Hslice He1 He2".
+     iApply (imp_EArrayUnsafeGet2 with "[He1] He2").
+     { iApply (imp_mono_ret with "He1").
+       iIntros (?) "->". iFrame "#".
+       instantiate (1 := (λ a', ⌜a' = a⌝)%I). done. }
+     iIntros (? ?) "-> ->".
+     iFrame "#".
+     iFrame "%". iFrame.
+     iIntros "!> $". done.
+   Qed.
+
+   Lemma imp_EArrayGet `{Encode A} {ζ} a (k n : Z) (i j : Z) dq (xs : list A) x e1 e2 :
+     representable i →
+     ⌜j ≤ i⌝ -∗
+     ⌜xs !! (i - j)%Z = Some x⌝ -∗
+     isArray a n -∗
+     ▷ isSlice dq a j xs -∗
+     imp^{ι} eval η e1 @ E <|Ψ|> ⟨⟨ ζ ⟩⟩ {{ λ a', ⌜a' = a⌝ }} -∗
+     imp^{ι} eval η e2 @ E <|Ψ|> ⟨⟨ ζ ⟩⟩ {{ λ i', ⌜i' = i⌝ }} -∗
+     imp^{ι} eval η (EArrayGet e1 e2) @ E <|Ψ|>
+       ⟨⟨ λ e, ζ e ∨ ⌜e = VException (Invalid_argument "index out of bounds")⌝ ∧ ⌜(i < 0 ∨ i >= n)%Z⌝ ⟩⟩
+       {{ λ v, ⌜v = x⌝ ∗ isSlice dq a j xs }}.
+   Proof.
+     iIntros (Hrepr Hi Hlookup) "#Harr Hslice He1 He2". simpl_eval.
+     iDestruct "Harr" as "(%ls & -> & %Heq & %Hbound)".
+
+     iApply (imp_Par _ _ _ _ _ _ (pfbind inject2
+               (λ '((ls0, i0) : list loc * int),
+                  match ls0 !! signed i0 with
+                  | Some l => load l
+                  | None => throw (invalid_argument "index out of bounds")
+                  end)) with "[He1] [He2]").
+     { rewrite /as_array.
+       iApply (imp_bind _ _ (λ v, val_as_array v) with "He1").
+       iIntros (?) "->".
+       iApply (imp_ret ls ls).
+       instantiate (1 := Build_Observe (list loc) _ (list loc) id). reflexivity.
+       instantiate (1 := (λ ls', ⌜ls' = ls⌝)%I). done. }
+     { rewrite /as_int.
+       iApply (imp_bind _ _ (λ v, val_as_int v) with "He2").
+       iIntros (?) "->".
+       iApply (imp_ret (repr i) i).
+       instantiate (1 := Build_Observe (Z) _ (int) repr). reflexivity.
+       instantiate (1 := (λ i', ⌜i' = i⌝)%I). done. }
+     iSplit; last iSplit.
+     { iIntros (e) "Hζ !>".
+       iApply (imp_throw with "[Hζ]"). by iLeft. }
+     { iIntros (e) "Hζ !>".
+       iApply (imp_throw with "[Hζ]"). by iLeft. }
+     iIntros (? ?) "-> -> !>".
+     rewrite /continue /= bind_ret.
+
+     iDestruct "Hslice" as "(% & %Heq' & %Hlen & Hslice)".
+     inversion Heq'; subst ls0; clear Heq'.
+
+     rewrite signed_repr; last assumption.
+
+     case (decide (0 ≤ i < n)); [ intros in_bounds | intros not_in_bounds ].
+     -
+
+       (* Decompose [ls] into [lj ++ slice ++ _]. *)
+       pose proof (cut_out_slice j (length xs) ls ltac:(lia) ltac:(lia))
+         as (lj & slice & lextra & Hls & Hj & Hslice).
+       (* Turn [take _ (drop _ ls)] into [slice]. *)
+       replace (Z.to_nat j) with (length lj) by lia.
+       rewrite {1}Hls drop_app_length.
+       replace (length xs) with (length slice) by lia.
+       rewrite take_app_length.
+
+       rewrite /lookup /list_lookup_Z in Hlookup.
+       assert (i - j <? 0 = false) as Heqf by lia.
+       rewrite Heqf in Hlookup.
+
+       assert (i - j < length xs).
+       { pose proof (lookup_lt_Some xs (Z.to_nat (i - j)) _ Hlookup). lia. }
+
+       (* [Decompose [xs] intl [xk ++ x :: _]. *)
+       pose proof (list_elem_of_split_length xs (Z.to_nat (i - j)) x Hlookup)
+         as (xk & xrest & Hxs & Hxk).
+       rewrite {1}Hxs.
+
+       (* Inversions on [Hslice] gives us that
+        [slice] = [slicek ++ l :: _]. *)
+       iDestruct (big_sepL2_app_inv_r with "Hslice")
+         as "(%slicek & %slice' & -> & Hslice1 & Hslice2)".
+       iDestruct (big_sepL2_cons_inv_r with "Hslice2") as
+         "(%l & %slicerest & -> & Hl & Hslice2)".
+
+       (* We can now prove that [ls !! Z.to_nat i] = [Some l]. *)
+       rewrite /lookup /list_lookup_Z.
+       assert (i <? 0 = false) as -> by lia.
+       rewrite {1}Hls lookup_app_r; last lia.
+       replace (Z.to_nat i - length lj)%nat with (Z.to_nat (i - j)) by lia.
+       rewrite <- app_assoc. iPoseProof (big_sepL2_length with "Hslice1") as "%Hleneq".
+       rewrite list_lookup_middle; last lia.
+
+       iApply (imp_load with "Hl").
+       rewrite /continue; iIntros "!> Hl /=".
+       iApply imp_ret. encode. iSplit; first auto.
+       iCombine ("Hl Hslice2") as "Hslice2".
+       iPoseProof (big_sepL2_cons (λ _ l' x', pointsto l' dq (V #x')) with "Hslice2") as "Hslice2".
+       iPoseProof (big_sepL2_app with "Hslice1 Hslice2") as "Hslice".
+       iExists ls. iSplit; first auto. iSplit.
+       { iPureIntro. lia. }
+       replace (Z.to_nat j) with (length lj) by lia.
+       rewrite {1}Hls drop_app_length.
+       replace (length xs) with (length (slicek ++ l :: slicerest)) by lia.
+       rewrite take_app_length.
+       rewrite Hxs.
+       iApply "Hslice".
+
+     - assert (i < 0 ∨ i >= n) as Hnbounds by lia.
+       rewrite /lookup /list_lookup_Z.
+       destruct Hnbounds.
+       + assert (i <? 0 = true) as -> by lia.
+         iApply imp_throw.
+         iRight. auto.
+       + assert (i <?0 = false) as -> by lia.
+         rewrite lookup_ge_None_2; last lia.
+         iApply imp_throw.
+         iRight. auto.
+   Qed.
 
 
 End array_reasoning.
